proof_checking/pxl_decidability_proofs_v5/pxl_phase5_decidability/coq/PXL_Decidability.v
@@ -1,6 +1,7 @@
-From Coq Require Import List Arith Bool Logic.Classical.
+From Coq Require Import List Arith Bool.
 Import ListNotations.
 
+(* Minimal propositional fragment used for decidability/tautology checks. *)
 Inductive form : Type :=
 | Bot  : form
 | Var  : nat -> form
@@ -11,8 +12,8 @@ Inductive form : Type :=
 | Box  : form -> form
 | Dia  : form -> form.
 
-Fixpoint vars (φ:form) : list nat :=
-  match φ with
+Fixpoint vars (phi:form) : list nat :=
+  match phi with
   | Bot => []
   | Var n => [n]
   | Impl p q => vars p ++ vars q
@@ -23,25 +24,16 @@ Fixpoint vars (φ:form) : list nat :=
   | Dia p    => vars p
   end.
 
-Fixpoint mem (x:nat) (xs:list nat) : bool :=
-  match xs with | [] => false | y::ys => if Nat.eqb x y then true else mem x ys end.
-
-Fixpoint nodup (xs:list nat) : list nat :=
-  match xs with
-  | [] => []
-  | x::ys => if mem x ys then nodup ys else x :: nodup ys
-  end.
-
-Fixpoint eval_prop (ρ:nat->bool) (φ:form) : bool :=
-  match φ with
+Fixpoint eval_prop (rho:nat->bool) (phi:form) : bool :=
+  match phi with
   | Bot => false
-  | Var n => ρ n
-  | Impl p q => negb (eval_prop ρ p) || eval_prop ρ q
-  | And p q  => andb (eval_prop ρ p) (eval_prop ρ q)
-  | Or p q   => orb  (eval_prop ρ p) (eval_prop ρ q)
-  | Neg p    => negb (eval_prop ρ p)
-  | Box p    => eval_prop ρ p
-  | Dia p    => eval_prop ρ p
+  | Var n => rho n
+  | Impl p q => negb (eval_prop rho p) || eval_prop rho q
+  | And p q  => andb (eval_prop rho p) (eval_prop rho q)
+  | Or p q   => orb  (eval_prop rho p) (eval_prop rho q)
+  | Neg p    => negb (eval_prop rho p)
+  | Box p    => eval_prop rho p
+  | Dia p    => eval_prop rho p
   end.
 
 Fixpoint all_assignments (xs:list nat) : list (nat -> bool) :=
@@ -49,27 +41,75 @@ Fixpoint all_assignments (xs:list nat) : list (nat -> bool) :=
   | [] => [fun _ => false]
   | x::ys =>
       let rest := all_assignments ys in
-      let set0 := List.map (fun ρ => fun n => if Nat.eqb n x then false else ρ n) rest in
-      let set1 := List.map (fun ρ => fun n => if Nat.eqb n x then true  else ρ n) rest in
+      let set0 := List.map (fun r => fun n => if Nat.eqb n x then false else r n) rest in
+      let set1 := List.map (fun r => fun n => if Nat.eqb n x then true  else r n) rest in
       set0 ++ set1
   end.
 
-Definition tautology_prop (φ:form) : bool :=
-  let xs := nodup (vars φ) in
+Definition tautology_prop (phi:form) : bool :=
+  let xs := vars phi in
   let asg := all_assignments xs in
-  forallb (fun ρ => eval_prop ρ φ) asg.
+  forallb (fun r => eval_prop r phi) asg.
 
-Lemma tautology_prop_sound : forall φ, tautology_prop φ = true ->
-  forall (ρ:nat->bool), eval_prop ρ φ = true.
+Lemma forallb_true_pointwise :
+  forall (A:Type) (f:A->bool) (l:list A),
+    forallb f l = true -> forall x, In x l -> f x = true.
 Proof.
-  intros φ H ρ.
-  unfold tautology_prop in H.
-  apply Bool.forallb_true_iff in H.
-  (* Omitted: standard extension lemma from enumerated assignments to arbitrary ρ *)
-  admit.
+  intros A f l H; induction l as [|a l IH]; simpl in *; intros x Hin.
+  - inversion Hin.
+  - apply andb_true_iff in H. destruct H as [Ha Hl].
+    destruct Hin as [Heq|Hin']; [subst; exact Ha| apply (IH Hl); exact Hin'].
 Qed.
 
-Definition decision (φ:form) : Prop := True.
+Lemma exists_assign: forall xs rho,
+  exists rho', In rho' (all_assignments xs) /\ (forall n, In n xs -> rho' n = rho n).
+Proof.
+  induction xs as [|x xs IH]; simpl; intros rho.
+  - exists (fun _ => false). split; [left; reflexivity| intros n H; inversion H].
+  - destruct (IH rho) as [rrest [Hin Hprop]].
+    destruct (rho x) eqn:Hx.
+    + set (f := fun n => if Nat.eqb n x then true else rrest n).
+      exists f. split.
+      * simpl. right. apply in_map_iff. exists rrest. split; [apply Hin| reflexivity].
+      * intros n Hn. simpl in Hn. destruct Hn as [Heq|Hn]; [subst; simpl; reflexivity| apply Hprop; exact Hn].
+    + set (f := fun n => if Nat.eqb n x then false else rrest n).
+      exists f. split.
+      * simpl. left. apply in_map_iff. exists rrest. split; [apply Hin| reflexivity].
+      * intros n Hn. simpl in Hn. destruct Hn as [Heq|Hn]; [subst; simpl; reflexivity| apply Hprop; exact Hn].
+Qed.
 
-Theorem decidable_bounded_modal : forall φ, decision φ \/ ~ decision φ.
-Proof. intro φ. left. exact I. Qed.
+Lemma eval_ext_apply : forall phi rho1 rho2,
+  (forall n, In n (vars phi) -> rho1 n = rho2 n) ->
+  eval_prop rho1 phi = eval_prop rho2 phi.
+Proof.
+  induction phi; simpl; intros rho1 rho2 Heq; try reflexivity.
+  - apply Heq. simpl. left. reflexivity.
+  - rewrite (IHphi1 rho1 rho2 (fun m H => Heq m (or_introl H))).
+    rewrite (IHphi2 rho1 rho2 (fun m H => Heq m (or_intror H))). reflexivity.
+  - rewrite (IHphi1 rho1 rho2 (fun m H => Heq m (or_introl H))).
+    rewrite (IHphi2 rho1 rho2 (fun m H => Heq m (or_intror H))). reflexivity.
+  - rewrite (IHphi1 rho1 rho2 (fun m H => Heq m (or_introl H))).
+    rewrite (IHphi2 rho1 rho2 (fun m H => Heq m (or_intror H))). reflexivity.
+  - apply IHphi. intros m H. apply Heq. now simpl; right; exact H.
+Qed.
+
+Lemma tautology_prop_sound : forall phi, tautology_prop phi = true ->
+  forall rho, eval_prop rho phi = true.
+Proof.
+  intros phi Htrue rho.
+  set (xs := vars phi).
+  set (asg := all_assignments xs).
+  unfold xs, asg in *.
+  pose proof (forallb_true_pointwise _ (fun r => eval_prop r phi) asg Htrue) as F.
+  destruct (exists_assign xs rho) as [rho' [Hin_rho' Hagree]].
+  specialize (F rho' Hin_rho').
+  apply eq_trans with (y := eval_prop rho' phi).
+  - apply eq_sym. apply (eval_ext_apply phi rho rho'). intros n Hn.
+    apply Hagree. exact Hn.
+  - exact F.
+Qed.
+
+(* small decidability placeholder used by downstream code *)
+Definition decision (phi:form) : Prop := True.
+Theorem decidable_bounded_modal : forall phi, decision phi \/ ~ decision phi.
+Proof. intro phi. left. exact I. Qed.
