proof_checking/pxl_decidability_proofs_v5/pxl_phase5_decidability/coq/TAUT_test.v
@@ -1,0 +1,5 @@
+From Coq Require Import List Bool.
+Import ListNotations.
+
+Lemma test_true_bool : True.
+Proof. exact I. Qed.
